code/experimental/P256/Hacl.Spec.P256.Ladder.fst
@@ -1,5 +1,9 @@
 module Hacl.Spec.P256.Ladder
 
+open FStar.HyperStack.All
+open FStar.HyperStack
+module ST = FStar.HyperStack.ST
+
 open Lib.IntTypes
 open Lib.Buffer
 
@@ -7,10 +11,14 @@ open Hacl.Spec.P256.Definitions
 open Hacl.Spec.P256.MontgomeryMultiplication
 open Hacl.Spec.P256.MontgomeryMultiplication.PointAdd 
 open Hacl.Spec.P256.MontgomeryMultiplication.PointDouble
+open Hacl.Impl.Curve25519.Field64.Core
 
 open FStar.Math.Lemmas
 open Lib.Sequence
 open Lib.ByteSequence
+
+
+let scalar = lbytes 32
 
 let ith_bit (k:lbytes 32) (i:nat{i < 256}) : uint64 =
 	let q = i / 8 in let r = size (i % 8) in
@@ -78,7 +86,7 @@ let montgomery_ladder_step0 r0 r1 =
   (r0, r1)
 
 
-val montgomery_ladder_step1: p: point_prime -> q: point_prime -> 
+val montgomery_ladder_step1_seq: p: point_prime -> q: point_prime -> 
   Tot (r: tuple2 point_prime point_prime 
     {
       let r0, r1 = r in 
@@ -126,7 +134,7 @@ val montgomery_ladder_step1: p: point_prime -> q: point_prime ->
   return R0 *)
 
 
-let montgomery_ladder_step1 r0 r1 = 
+let montgomery_ladder_step1_seq r0 r1 = 
   let r1 = point_add_seq r0 r1 in 
   let r0 = point_double_seq r0 in  
   (r0, r1)
@@ -156,12 +164,91 @@ let conditional_swap i p q =
   else
     (q, p)
 
+
+(*This code is taken from Curve25519, written by Polubelova M *)
+val lemma_cswap2_step:
+    bit:uint64{v bit <= 1}
+  -> p1:uint64
+  -> p2:uint64
+  -> Lemma (
+      let mask = u64 0 -. bit in
+      let dummy = mask &. (p1 ^. p2) in
+      let p1' = p1 ^. dummy in
+      let p2' = p2 ^. dummy in
+      if v bit = 1 then p1' == p2 /\ p2' == p1 else p1' == p1 /\ p2' == p2)
+let lemma_cswap2_step bit p1 p2 =
+  let mask = u64 0 -. bit in
+  assert (v bit == 0 ==> v mask == 0);
+  assert (v bit == 1 ==> v mask == pow2 64 - 1);
+  let dummy = mask &. (p1 ^. p2) in
+  logand_lemma mask (p1 ^. p2);
+  assert (v bit == 1 ==> v dummy == v (p1 ^. p2));
+  assert (v bit == 0 ==> v dummy == 0);
+  let p1' = p1 ^. dummy in
+  uintv_extensionality dummy (if v bit = 1 then (p1 ^. p2) else u64 0);
+  logxor_lemma p1 p2;
+  let p2' = p2 ^. dummy in
+  logxor_lemma p2 p1
+
+[@ CInline]
+val cswap: bit:uint64{v bit <= 1} -> p:point -> q:point
+  -> Stack unit
+    (requires fun h ->
+      live h p /\ live h q /\ (disjoint p q \/ p == q) /\
+           
+      as_nat h (gsub p (size 0) (size 4)) < prime /\ 
+      as_nat h (gsub p (size 4) (size 4)) < prime /\
+      as_nat h (gsub p (size 8) (size 4)) < prime /\
+	     
+      as_nat h (gsub q (size 0) (size 4)) < prime /\  
+      as_nat h (gsub q (size 4) (size 4)) < prime /\
+      as_nat h (gsub q (size 8) (size 4)) < prime
+)
+    (ensures  fun h0 _ h1 ->
+      modifies (loc p |+| loc q) h0 h1 /\
+      (let pBefore = as_seq h0 p in let qBefore = as_seq h0 q in 
+	let pAfter = as_seq h1 p in let qAfter = as_seq h1 q in 
+	let condP0, condP1 = conditional_swap bit pBefore qBefore  in 
+	condP0 == pAfter /\ condP1 == qAfter) /\ 
+
+      (v bit == 1 ==> as_seq h1 p == as_seq h0 q /\ as_seq h1 q == as_seq h0 p) /\
+      (v bit == 0 ==> as_seq h1 p == as_seq h0 p /\ as_seq h1 q == as_seq h0 q))
+
+
+let cswap bit p1 p2 =
+  let h0 = ST.get () in
+  let mask = u64 0 -. bit in
+
+  [@ inline_let]
+  let inv h1 (i:nat{i <= 12}) =
+    (forall (k:nat{k < i}).
+      if v bit = 1
+      then (as_seq h1 p1).[k] == (as_seq h0 p2).[k] /\ (as_seq h1 p2).[k] == (as_seq h0 p1).[k]
+      else (as_seq h1 p1).[k] == (as_seq h0 p1).[k] /\ (as_seq h1 p2).[k] == (as_seq h0 p2).[k]) /\
+    (forall (k:nat{i <= k /\ k < 12}).
+      (as_seq h1 p1).[k] == (as_seq h0 p1).[k] /\ (as_seq h1 p2).[k] == (as_seq h0 p2).[k]) /\
+    modifies (loc p1 |+| loc p2) h0 h1 in
+ 
+  Lib.Loops.for 0ul 12ul inv
+    (fun i ->
+      let dummy = mask &. (p1.(i) ^. p2.(i)) in
+      p1.(i) <- p1.(i) ^. dummy;
+      p2.(i) <- p2.(i) ^. dummy;
+      lemma_cswap2_step bit ((as_seq h0 p1).[v i]) ((as_seq h0 p2).[v i])
+    );
+  let h1 = ST.get () in
+  Lib.Sequence.eq_intro (as_seq h1 p1) (if v bit = 1 then as_seq h0 p2 else as_seq h0 p1);
+  Lib.Sequence.eq_intro (as_seq h1 p2) (if v bit = 1 then as_seq h0 p1 else as_seq h0 p2)
+
+
+
+
 #reset-options "--z3refresh --z3rlimit 100"
 
 val lemma_swaped_steps: p: point_prime -> q: point_prime -> 
   Lemma (
     let (afterSwapP, afterSwapQ) = swap p q in 
-    let p1, q1 = montgomery_ladder_step1 afterSwapP afterSwapQ in 
+    let p1, q1 = montgomery_ladder_step1_seq afterSwapP afterSwapQ in 
     let p2, q2 = swap p1 q1 in 
     let r0, r1 = montgomery_ladder_step0 p q in 
     p2 == r0 /\ q2 == r1)
@@ -173,7 +260,7 @@ let lemma_swaped_steps p q =
   
   let afterSwapP, afterSwapQ = swap p q in 
     assert(afterSwapP == q /\ afterSwapQ == p);
-  let (p1, q1) = montgomery_ladder_step1 afterSwapP afterSwapQ in 
+  let (p1, q1) = montgomery_ladder_step1_seq afterSwapP afterSwapQ in 
     assert(q1 == point_add_seq q p);
     assert(p1 == point_double_seq q);
   let (p2, q2) = swap p1 q1 in 
@@ -188,9 +275,10 @@ val montgomery_ladder_step_swap: p: point_prime -> q: point_prime -> k: scalar -
    
 
 let montgomery_ladder_step_swap p q k i = 
-  let bit = ith_bit k i in 
+  let bit = 255 - i in 
+  let bit = ith_bit k bit in 
   let p0, q0 = conditional_swap bit p q in 
-  let p1, q1 = montgomery_ladder_step1 p0 q0 in 
+  let p1, q1 = montgomery_ladder_step1_seq p0 q0 in 
   let p2, q2 = conditional_swap bit p1 q1 in
    (p2, q2)  
  
